started lemma

fstar/Storage.fst
@@ -1,15 +1,53 @@
 module Storage
 
-type value a b c =
-  | Mtst : value a b c
-  | Var : (v : a) -> value a b c
-  | Store : (st : value a b c) -> (k : either b c) -> (v : value a b c) -> value a b c
+type value a b =
+  | Mtst : value a b
+  | Var : (v : a) -> value a b
+  | Store : (st : value a b) -> (k : b) -> (v : value a b) -> value a b
 
-let rec save #a (#b : eqtype) (#c : eqtype)  (st : value a b c) (flds : list (either b c))  (v : value a b c)
-  : Tot (value a b c) (decreases st)
+let rec save #a (#b : eqtype) (st : value a b) (flds : list b)  (v : value a b)
+  : Tot (value a b) (decreases %[flds;st])
   = match st, flds with
     | Mtst, [] -> v
     | Mtst, k :: xs -> Store Mtst k (save Mtst xs v)
     | Var _, _ -> v
     | Store st x v', [] -> Store st x v'
     | Store st k v', k' :: ys -> if k = k' then Store st k (save v ys v') else Store (save st (k' :: ys) v') k v
+
+let rec select #a (#b : eqtype) (st : value a b) (n : b) : value a b
+  = match st with
+  | Mtst -> Mtst
+  | Var st -> Mtst
+  | Store st k v -> if k = n then v else select st k
+
+let rec isStruct #a #b (st : value a b) : bool
+  = match st with
+  | Mtst -> true
+  | Var _ -> false
+  | Store st _ Mtst -> isStruct st
+  | Store st _ (Var _) -> isStruct st
+  | Store st _ (Store v x v2) -> isStruct st && isStruct (Store v x v2)
+
+// let rec isStructInside #a #b (st : value a b) (k : b) (v : value a b) :
+//   Lemma (requires isStruct (Store st k v))
+//     (ensures isStruct st)
+//   = match st with
+//   | Mtst -> _
+//   | Var _ -> _
+//   | Store _ _ _ -> _
+
+
+let rec select_save #a (#b : eqtype) (st : value a b) (k : b) (path : list b) (v : value a b) (k' : b)
+  : Lemma (requires isStruct st)
+    (ensures select (save st (k :: path) v) k' == (if k = k' then save (select st k') path v else select st k'))
+  = match st with
+    | Mtst -> _
+    | Var _ -> _
+    | Store st' k''' v' ->
+      // isStructInside st' k''' v';
+      select_save st' k path v k;
+      select_save st' k path v k';
+      assume k''' == k;
+      assume k == k';
+      assert ((if k = k' then save (select st k') path v else select st k') == save (select st k') path v);
+      _
